src/Flutterbye.Seq.Filter.fst
@@ -1,6 +1,6 @@
 (*--build-config
    options:--admit_fsi FStar.Seq --admit_fsi Flutterbye.Seq.Mem;
-   other-files:seq.fsi Flutterbye.Seq.Mem.fsi
+   other-files:seq.fsi Flutterbye.Seq.Mem.fsi Flutterbye.Seq.Filter.fsi
 --*)
 
 // $legal:614:
@@ -22,115 +22,116 @@
 // ,$
 
 module Flutterbye.Seq.Filter
-   open FStar.Seq
-   open Flutterbye.Seq.Mem
+open FStar.Seq
+open Flutterbye.Seq.Mem
 
-   val filter__loop:
-      // predicate; if false, then the element is discarded from the sequence.
-      ('a -> Tot bool)
-      // input sequence
-      -> s: seq 'a
-      // index of element being reduced with (length s) as representing
-      // the base case.
-      -> i: nat{i <= length s}
-      // accumulator; in this case, the output sequence.
-      -> c: seq 'a
-      -> Tot (seq 'a)
-         (decreases (length s - i))
-   let rec filter__loop p s i c =
-      if i = length s then
-         c
-      else
-         let a = index s i in
-         let c' =
-            if p a then
-               append c (create 1 a)
-            else
-               c in
-         filter__loop p s (i + 1) c'
+val filter__loop:
+   // predicate; if false, then the element is discarded from the sequence.
+   ('a -> Tot bool)
+   // input sequence
+   -> s:seq 'a
+   // index of element being reduced with (length s) as representing
+   // the base case.
+   -> i:nat{i <= length s}
+   // accumulator; in this case, the output sequence.
+   -> c:seq 'a
+   -> Tot (seq 'a)
+      (decreases (length s - i))
+let rec filter__loop p s i c =
+   if i = length s then
+      c
+   else
+      let a = index s i in
+      let c' =
+         if p a then
+            append c (create 1 a)
+         else
+            c in
+      filter__loop p s (i + 1) c'
 
-   let filter p s =
-      filter__loop p s 0 createEmpty
+let filter p s =
+   filter__loop p s 0 createEmpty
 
-   val lemma__length__loop:
-      p: ('a -> Tot bool) ->
-      s: seq 'a ->
-      i: nat{i <= length s} ->
-      c: seq 'a ->
-      Lemma
-         (requires (length c <= i))
-         (ensures (length (filter__loop p s i c) <= length s))
-         (decreases (length s - i))
-   let rec lemma__length__loop p s i c =
-      if i = length s then
-         ()
-      else
-         let a = index s i in
-         let c' =
-            if p a then
-               append c (create 1 a)
-            else
-               c in
-         lemma__length__loop p s (i + 1) c'
+val lemma__length__loop:
+   p: ('a -> Tot bool)
+   -> s:seq 'a
+   -> i:nat{i <= length s}
+   -> c:seq 'a
+   -> Lemma
+      (requires (length c <= i))
+      (ensures (length (filter__loop p s i c) <= length s))
+      (decreases (length s - i))
+let rec lemma__length__loop p s i c =
+   if i = length s then
+      ()
+   else
+      let a = index s i in
+      let c' =
+         if p a then
+            append c (create 1 a)
+         else
+            c in
+      lemma__length__loop p s (i + 1) c'
 
-   let lemma__length p s =
-      lemma__length__loop p s 0 createEmpty
+let lemma__length p s =
+   lemma__length__loop p s 0 createEmpty
 
-   val lemma__predicate__loop:
-      p: ('a -> Tot bool)
-      -> s: seq 'a
-      -> i: nat{i <= length s}
-      // accumulator-- in this case, a filtered sequence being constructed.
-      -> c: seq 'a
-      // free variable (forall)
-      -> j: nat
-      -> Lemma
-         (requires
-            (forall k.
-               0 <= k && k < length c ==> p (index c k)))
-         (ensures
-            (j < length (filter__loop p s i c)
-            ==> p (index (filter__loop p s i c) j)))
-         (decreases (length s - i))
-   let rec lemma__predicate__loop p s i c j =
-      if i = length s then
-         ()
-      else
-         let a = index s i in
-         let c' =
-            if p a then
-               append c (create 1 a)
-            else
-               c in
-         lemma__predicate__loop p s (i + 1) c' j
+val lemma__predicate__loop:
+   p: ('a -> Tot bool)
+   -> s:seq 'a
+   -> i:nat{i <= length s}
+   // accumulator-- in this case, a filtered sequence being constructed.
+   -> c:seq 'a
+   // free variable (forall)
+   -> j:nat
+   -> Lemma
+      (requires
+         (forall k.
+            0 <= k && k < length c ==> p (index c k)))
+      (ensures
+         (j < length (filter__loop p s i c)
+         ==> p (index (filter__loop p s i c) j)))
+      (decreases (length s - i))
+let rec lemma__predicate__loop p s i c j =
+   if i = length s then
+      ()
+   else
+      let a = index s i in
+      let c' =
+         if p a then
+            append c (create 1 a)
+         else
+            c in
+      lemma__predicate__loop p s (i + 1) c' j
 
-   let lemma__predicate p s i =
-      lemma__predicate__loop p s 0 createEmpty i
+let lemma__predicate p s i =
+   lemma__predicate__loop p s 0 createEmpty i
 
-   val lemma__mem__loop:
-      p: ('a -> Tot bool)
-      -> s: seq 'a
-      -> i: nat{i <= length s}
-      -> c: seq 'a
-      -> Lemma
-         (requires
-            (forall j.
-               (0 <= j && j < length c) ==> (mem (index c j) s)))
-         (ensures
-            (forall j.
-               (0 <= j && j < length (filter__loop p s i c)) ==> (mem (index (filter__loop p s i c) j) s)))
-         (decreases (length s - i))
-   let rec lemma__mem__loop p s i c =
-      if i = length s then
-         ()
-      else
-         let a = index s i in
-         let c' =
-            if p a then
-               append c (create 1 a)
-            else
-               c in
-         lemma__mem__loop p s (i + 1) c'
+val lemma__mem__loop:
+   p: ('a -> Tot bool)
+   -> s:seq 'a
+   -> i:nat{i <= length s}
+   -> c:seq 'a
+   -> Lemma
+      (requires
+         (forall (j:nat).
+            (j < length c) ==> (mem (index c j) s)))
+      (ensures
+         (forall (j:nat).
+            (j < length (filter__loop p s i c)) ==>
+               (mem (index (filter__loop p s i c) j) s)))
+      (decreases (length s - i))
+let rec lemma__mem__loop p s i c =
+   if i = length s then
+      ()
+   else
+      let a = index s i in
+      let c' =
+         if p a then
+            append c (create 1 a)
+         else
+            c in
+      lemma__mem__loop p s (i + 1) c'
 
-   let lemma__mem p s =
-      lemma__mem__loop p s 0 createEmpty
+let lemma__mem p s =
+   lemma__mem__loop p s 0 createEmpty
